TC.Instrumentable.fst
@@ -1,0 +1,17 @@
+module TC.Instrumentable
+
+open FStar.Tactics
+open FStar.Tactics.Typeclasses
+
+open TC.Export
+open TC.MLify
+
+class instrumentable (t:Type) = { 
+  a: Type; b: Type;
+  a_c: ml a;
+  b_c: ml b;
+  start_type : Type;
+  start_type_c : ml_arrow start_type;
+  (** be careful to not use reify while writing this instrument **)
+  instrument : start_type -> t
+} 
