io/TC.Instrumentable.IIO.fst
@@ -1,0 +1,66 @@
+module TC.Instrumentable.IIO
+
+open FStar.List.Tot
+open FStar.Tactics
+open FStar.Tactics.Typeclasses
+
+open Free.IO
+open Common
+open TC.Export
+open TC.Monitorable
+open TC.MLify
+include TC.Instrumentable
+open DM.IIO
+
+
+let extract_local_trace (h':trace) (pi:monitorable_prop) :
+  IIO trace pi
+    (requires (fun h -> h' `suffix_of` h))
+    (ensures (fun h lt' lt ->
+      lt == [] /\
+      h == (apply_changes h' lt'))) =
+  let h = get_trace () in
+  suffix_of_length h' h;
+  let n : nat = (List.length h) - (List.length h') in
+  let (lt', ht) = List.Tot.Base.splitAt n h in
+  lemma_splitAt_equal n h;
+  lemma_splitAt_suffix h h';
+  List.Tot.Properties.rev_involutive lt';
+  assert (h == apply_changes h' (List.rev lt'));
+  List.rev lt'
+
+let enforce_post
+  (#t1 #t2:Type)
+  (pi:monitorable_prop)
+  (pre:t1 -> trace -> Type0)
+  (post:t1 -> trace -> (r:maybe t2) -> trace -> (b:Type0{r == Inr Contract_failure ==> b}))
+  {| post_c:monitorable_post pre post pi |}
+  (f:t1 -> IIO (maybe t2) pi (fun _ -> True) (fun _ _ _ -> True))
+  (x:t1) :
+  IIO (maybe t2) pi (pre x) (post x) =
+  let h = get_trace () in
+  let r : maybe t2 = f x in
+  Classical.forall_intro (lemma_suffixOf_append h);
+  let lt = extract_local_trace h pi in
+  Classical.forall_intro_2 (Classical.move_requires_2 (lemma_append_rev_inv_tail h));
+  if post_c.result_check x h r lt then begin
+    assume (enforced_globally pi ((rev lt)@h) ==> enforced_locally pi h lt);
+    r
+  end else Inr Contract_failure
+
+instance instrumentable_IIO 
+  (#t1:Type) (#t2:Type) {| d1:ml t1 |} {| d2:ml t2 |}
+  (pre : t1 -> trace -> Type0)
+  (** it must be `maybe t2` because needs the ability to fail **)
+  (post : t1 -> trace -> (r:maybe t2) -> trace -> (b:Type0{r == Inr Contract_failure ==> b}))
+  (pi : monitorable_prop) {| post_c:monitorable_post pre post pi |} : 
+  instrumentable ((x:t1) -> IIO (maybe t2) pi (pre x) (post x)) =
+  { a = t1; b = t2; a_c = d1; b_c = d2;
+    start_type = t1 -> Tot (maybe t2);
+    start_type_c = ml_arrow_tot_1 t1 (maybe t2);
+    instrument = (fun (f:t1 -> Tot (maybe t2)) ->
+      (** automatic lift from Pure to IIO. pi is enforced because a Pure 
+        computation has an empty trace **)
+      let f' : t1 -> IIO (maybe t2) pi (fun _ -> True) (fun _ _ _ -> True) = f in 
+      enforce_post #t1 #t2 pi pre post #post_c f')
+  }
